Show that occuring arguments are finite

CFGraph/AbsCFComp.thy
@@ -68,6 +68,17 @@ fixrec abs_R :: "('c::contour \<afstate> + 'c \<acstate>) discr \<rightarrow> ('
 definition maps_over :: "'a::type set \<Rightarrow> 'b::type set \<Rightarrow> ('a \<rightharpoonup> 'b) set"
   where "maps_over A B = {m. dom m \<subseteq> A \<and> ran m \<subseteq> B}"
 
+lemma maps_over_empty[simp]:
+  "empty \<in> maps_over A B"
+unfolding maps_over_def by simp
+
+lemma maps_over_upd:
+  assumes "m \<in> maps_over A B"
+  and "v \<in> A" and "k \<in> B"
+shows "m(v \<mapsto> k) \<in> maps_over A B"
+  using assms unfolding maps_over_def
+  by (auto dest: subsetD[OF ran_upd])
+
 lemma maps_over_finite[intro]:
   assumes "finite A" and "finite B" shows "finite (maps_over A B)"
 proof-
@@ -98,6 +109,32 @@ qed
 definition smaps_over :: "'a::type set \<Rightarrow> 'b::type set \<Rightarrow> ('a \<Rightarrow> 'b set) set"
   where "smaps_over A B = {m. sdom m \<subseteq> A \<and> sran m \<subseteq> B}"
 
+lemma smaps_over_empty[simp]:
+  "{}. \<in> smaps_over A B"
+unfolding smaps_over_def by simp
+
+lemma smaps_over_singleton:
+  assumes "k \<in> A" and "vs \<subseteq> B"
+shows "{k := vs}. \<in> smaps_over A B"
+  using assms unfolding smaps_over_def
+  by(auto dest: subsetD[OF sdom_singleton])
+
+lemma smaps_over_un:
+  assumes "m1 \<in> smaps_over A B" and "m2 \<in> smaps_over A B"
+  shows "m1 \<union>. m2 \<in> smaps_over A B"
+using assms unfolding smaps_over_def
+by (auto simp add:smap_union_def)
+
+lemma smaps_over_Union:
+  assumes "set ms \<subseteq> smaps_over A B"
+  shows "\<Union>.ms \<in> smaps_over A B"
+using assms
+by (induct ms)(auto intro: smaps_over_un)
+
+lemma smaps_over_im:
+ "\<lbrakk> f \<in> m a ; m \<in> smaps_over A B \<rbrakk> \<Longrightarrow> f \<in> B"
+unfolding smaps_over_def by (auto simp add:sran_def)
+
 lemma smaps_over_finite[intro]: 
   assumes "finite A" and "finite B" shows "finite (smaps_over A B)"
 proof-
@@ -125,11 +162,8 @@ proof-
     by (rule finite_imageD[OF _ subset_inj_on[OF inj_smap_graph subset_UNIV]])
 qed
 
-definition prim_poss :: "prog \<Rightarrow> prim set"
-  where "prim_poss p = (Plus ` labels p \<union> { prim.If p1 p1 | p1 p2 .  p1 \<in> labels p \<and> p2 \<in> labels p})"
-
 definition proc_poss :: "prog \<Rightarrow> 'c::contour proc set"
-  where "proc_poss p = PC ` (lambdas p \<times> maps_over (labels p) UNIV) \<union> PP ` prim_poss p \<union> {AStop}"
+  where "proc_poss p = PC ` (lambdas p \<times> maps_over (labels p) UNIV) \<union> PP ` prims p \<union> {AStop}"
 
 definition fstate_poss :: "prog \<Rightarrow> 'c::contour a_fstate set"
   where "fstate_poss p = (proc_poss p \<times> NList (Pow (proc_poss p)) (call_list_lengths p) \<times> smaps_over (vars p \<times> UNIV) (proc_poss p) \<times> UNIV)"
@@ -137,12 +171,236 @@ definition fstate_poss :: "prog \<Rightarrow> 'c::contour a_fstate set"
 definition cstate_poss :: "prog \<Rightarrow> 'c::contour a_cstate set"
   where "cstate_poss p = (calls p \<times> maps_over (labels p) UNIV \<times> smaps_over (vars p \<times> UNIV) (proc_poss p) \<times> UNIV)"
 
-definition arg_poss :: "prog \<Rightarrow> ('c::contour a_fstate + 'c a_cstate) set"
-  where "arg_poss p = fstate_poss p <+> cstate_poss p"
+definition arg_poss :: "prog \<Rightarrow> ('c::contour a_fstate + 'c a_cstate) discr set"
+  where "arg_poss p = Discr ` (fstate_poss p <+> cstate_poss p)"
 
 lemma finite_arg_space: "finite (arg_poss p)"
-  unfolding prim_poss_def and arg_poss_def and cstate_poss_def and fstate_poss_def and proc_poss_def
+  unfolding arg_poss_def and cstate_poss_def and fstate_poss_def and proc_poss_def
   by (auto intro!: finite_cartesian_product finite_imageI maps_over_finite smaps_over_finite contour_finite finite_Nlist)
+
+lemma adm_subset: "cont (\<lambda>x. f x) \<Longrightarrow>  adm (\<lambda>x. f x \<subseteq> S)"
+by (subst sqsubset_is_subset[THEN sym], intro adm_lemmas cont2cont)
+
+lemma evalV_possible:
+  assumes f: "f \<in> \<aA> d \<beta> ve"
+  and d: "d \<in> vals p"
+  and ve: "ve \<in> smaps_over (vars p \<times> UNIV) (proc_poss p)"
+  and \<beta>: "\<beta> \<in> maps_over (labels p) UNIV"
+shows "f \<in> proc_poss p"
+proof (cases "(d,\<beta>,ve)" rule: evalV_a.cases)
+case (1 cl \<beta>' ve')
+  thus ?thesis using f by auto next
+case (2 prim \<beta>' ve')
+  thus ?thesis using d f
+    by (auto dest: vals1 simp add:proc_poss_def)
+next
+case (3 l var \<beta>' ve') 
+  thus ?thesis using f d smaps_over_im[OF _ ve]
+  by (auto split:option.split_asm dest: vals2)
+next
+case (4 l \<beta> ve)
+  thus ?thesis using f d \<beta>
+  by (auto dest!: vals3 simp add:proc_poss_def)
+qed
+
+
+lemma arg_space_complete:
+  "state \<in> arg_poss p \<Longrightarrow> abs_R\<cdot>state \<subseteq> arg_poss p"
+proof(induct rule: abs_R.induct[case_names Admissibility Bot Step])
+case Admissibility show ?case
+   by (intro adm_lemmas adm_subset cont2cont)
+next
+case Bot show ?case by simp next
+case (Step abs_R) 
+  note state = Step(2)
+  show ?case
+  proof (cases state)
+  case (Discr state') show ?thesis
+   proof (cases state')
+     case (Inl fstate) show ?thesis
+     using Inl Discr state
+     proof (cases fstate rule:a_fstate_case)
+     apply_end(auto)
+     (* Lambda *)
+     fix l vs c \<beta> as ve b
+     assume "Discr (Inl (PC (Lambda l vs c, \<beta>), as, ve, b)) \<in> arg_poss p"
+       hence lam: "Lambda l vs c \<in> lambdas p"
+       and  beta: "\<beta> \<in> maps_over (labels p) UNIV "
+       and  ve: "ve \<in> smaps_over (vars p \<times> UNIV) (proc_poss p)"
+       and  as: "as \<in> NList (Pow (proc_poss p)) (call_list_lengths p)"
+       unfolding arg_poss_def fstate_poss_def proc_poss_def by auto
+
+     from lam have "c \<in> calls p"
+       by (rule lambdas1)
+
+     moreover
+     from lam have "l \<in> labels p"
+       by (rule lambdas2)
+     with beta have "\<beta>(l \<mapsto> b) \<in> maps_over (labels p) UNIV"
+       by (rule maps_over_upd, auto)
+
+     moreover
+     from lam have vs: "set vs \<subseteq> vars p" by (rule lambdas3)
+     from as have "\<forall> x \<in> set as. x \<in> Pow (proc_poss p)"
+        unfolding NList_def nList_def by auto
+     with vs have "ve \<union>. \<Union>.map (\<lambda>(v, y). { (v, b) := y}.) (zip vs as)
+       \<in> smaps_over (vars p \<times> UNIV) (proc_poss p)" (is "?ve' \<in> _")
+       by (auto intro!: smaps_over_un[OF ve] smaps_over_Union smaps_over_singleton)
+          (auto simp add:set_zip)
+
+     ultimately
+     have "(c, \<beta>(l \<mapsto> b), ?ve', b) \<in> cstate_poss p" (is "?cstate \<in> _")
+       unfolding cstate_poss_def by simp
+     thus "Discr (Inr ?cstate) \<in> arg_poss p"
+       unfolding arg_poss_def by auto
+     next
+
+     (* Plus *)
+     fix ve b l v1 v2 cnts cnt
+     assume "Discr (Inl (PP (prim.Plus l), [v1, v2, cnts], ve, b)) \<in> arg_poss p"
+         and "cnt \<in> cnts"
+     hence "cnt \<in> proc_poss p" 
+         and "ve \<in> smaps_over (vars p \<times> UNIV) (proc_poss p)"
+       unfolding arg_poss_def fstate_poss_def NList_def nList_def
+       by auto
+     moreover
+     have "[{}] \<in> NList (Pow (proc_poss p)) (call_list_lengths p)"
+       unfolding call_list_lengths_def NList_def nList_def by auto
+     ultimately
+     have "(cnt, [{}], ve, \<anb> b l) \<in> fstate_poss p"
+       unfolding fstate_poss_def by auto
+     thus "Discr (Inl (cnt, [{}], ve, \<anb> b l)) \<in> arg_poss p"
+       unfolding arg_poss_def by auto
+     next
+  
+     (* If True *)
+     fix ve b l1 l2 v cntst cntsf cnt
+     assume "Discr (Inl (PP (prim.If l1 l2), [v, cntst, cntsf], ve, b)) \<in> arg_poss p"
+         and "cnt \<in> cntst"
+     hence "cnt \<in> proc_poss p"
+         and "ve \<in> smaps_over (vars p \<times> UNIV) (proc_poss p)"
+       unfolding arg_poss_def fstate_poss_def NList_def nList_def
+       by auto
+     moreover
+     have "[] \<in> NList (Pow (proc_poss p)) (call_list_lengths p)"
+       unfolding call_list_lengths_def NList_def nList_def by auto
+     ultimately
+     have "(cnt, [], ve, \<anb> b l1) \<in> fstate_poss p"
+       unfolding fstate_poss_def by auto
+     thus "Discr (Inl (cnt, [], ve, \<anb> b l1)) \<in> arg_poss p"
+       unfolding arg_poss_def by auto
+     next
+  
+     (* If False *)
+     fix ve b l1 l2 v cntst cntsf cnt
+     assume "Discr (Inl (PP (prim.If l1 l2), [v, cntst, cntsf], ve, b)) \<in> arg_poss p"
+         and "cnt \<in> cntsf"
+     hence "cnt \<in> proc_poss p"
+         and "ve \<in> smaps_over (vars p \<times> UNIV) (proc_poss p)"
+       unfolding arg_poss_def fstate_poss_def NList_def nList_def
+       by auto
+     moreover
+     have "[] \<in> NList (Pow (proc_poss p)) (call_list_lengths p)"
+       unfolding call_list_lengths_def NList_def nList_def by auto
+     ultimately
+     have "(cnt, [], ve, \<anb> b l2) \<in> fstate_poss p"
+       unfolding fstate_poss_def by auto
+     thus "Discr (Inl (cnt, [], ve, \<anb> b l2)) \<in> arg_poss p"
+       unfolding arg_poss_def by auto
+    qed
+  next
+  case (Inr cstate)
+  show ?thesis proof(cases cstate rule: prod_cases4)
+   case (fields c \<beta> ve b)
+   show ?thesis using Discr Inr fields state proof(cases c, auto simp add:HOL.Let_def simp del:evalV_a.simps)
+     (* App *)
+     fix l d ds f
+     assume arg: "Discr (Inr (App l d ds, \<beta>, ve, b)) \<in> arg_poss p"
+       and f: "f \<in> \<aA> d \<beta> ve"
+     hence c: "App l d ds \<in> calls p"
+       and d: "d \<in> vals p"
+       and ds: "set ds \<subseteq> vals p"
+       and beta: "\<beta> \<in> maps_over (labels p) UNIV"
+       and ve: "ve \<in> smaps_over (vars p \<times> UNIV) (proc_poss p)"
+     by (auto simp add: arg_poss_def cstate_poss_def call_list_lengths_def dest: app1 app2)
+
+     have len: "length ds \<in> call_list_lengths p"
+       by (auto intro: rev_image_eqI[OF c] simp add: call_list_lengths_def)
+
+     have "f \<in> proc_poss p"
+       using f d ve beta by (rule evalV_possible)
+     moreover
+     have "map (\<lambda>v. \<aA> v \<beta> ve) ds \<in> NList (Pow (proc_poss p)) (call_list_lengths p)"
+       using ds len
+       unfolding NList_def by (auto simp add:nList_def intro!: evalV_possible[OF _ _ ve beta])
+     ultimately 
+     have "(f, map (\<lambda>v. \<aA> v \<beta> ve) ds, ve, \<anb> b l) \<in> fstate_poss p" (is "?fstate \<in> _")
+       using ve 
+       unfolding fstate_poss_def by simp
+     thus "Discr (Inl ?fstate) \<in> arg_poss p"
+       unfolding arg_poss_def by auto
+
+   next
+     (* Let *)
+     fix l binds c'
+     assume arg: "Discr (Inr (Let l binds c', \<beta>, ve, b)) \<in> arg_poss p"
+     hence l: "l \<in> labels p"
+       and c': "c' \<in> calls p"
+       and vars: "fst ` set binds \<subseteq> vars p"
+       and ls: "snd ` set binds \<subseteq> lambdas p"
+       and beta: "\<beta> \<in> maps_over (labels p) UNIV"
+       and ve: "ve \<in> smaps_over (vars p \<times> UNIV) (proc_poss p)"
+     by (auto simp add: arg_poss_def cstate_poss_def call_list_lengths_def
+              dest:let1 let2 let3 let4)
+
+     have beta': "\<beta>(l \<mapsto> \<anb> b l) \<in> maps_over (labels p) UNIV" (is "?\<beta>' \<in> _")
+       by (auto intro: maps_over_upd[OF beta l])
+
+     moreover
+     have "ve \<union>. \<Union>.map (\<lambda>(v, lam). { (v, \<anb> b l) := \<aA> (L lam) (\<beta>(l \<mapsto> \<anb> b l)) ve }.)
+                binds
+       \<in> smaps_over (vars p \<times> UNIV) (proc_poss p)" (is "?ve' \<in> _")
+       using vars ls beta'
+       by (auto intro!: smaps_over_un[OF ve] smaps_over_Union)
+          (auto intro!:smaps_over_singleton simp add: proc_poss_def)
+
+     ultimately
+     have "(c', ?\<beta>', ?ve', \<anb> b l) \<in> cstate_poss p" (is "?cstate \<in> _")
+     using c' unfolding cstate_poss_def by simp
+     thus "Discr (Inr ?cstate) \<in> arg_poss p"
+       unfolding arg_poss_def by auto
+   qed
+ qed
+qed
+qed
+qed
+
+lemma UN_iterate_less: 
+  assumes start: "x \<in> S"
+  and step: "\<And>y. y\<subseteq>S \<Longrightarrow> (f\<cdot>y) \<subseteq> S"
+  shows "(\<Union>i. iterate i\<cdot>f\<cdot>{x}) \<subseteq> S"
+proof- {
+  fix i
+  have "iterate i\<cdot>f\<cdot>{x} \<subseteq> S"
+  proof(induct i)
+    case 0 show ?case using `x \<in> S` by simp next
+    case (Suc i) thus ?case using step[of "iterate i\<cdot>f\<cdot>{x}"] by simp
+  qed
+  } thus ?thesis by auto
+qed
+
+lemma arg_space_complete_ps: "states \<subseteq> arg_poss p \<Longrightarrow> (\<^ps> abs_R)\<cdot>states \<subseteq> arg_poss p"
+using arg_space_complete unfolding powerset_lift_def by auto
+
+lemma args_finite: "finite (\<Union>i. iterate i\<cdot>(\<^ps> abs_R)\<cdot>{Discr (Inl
+     (contents (\<aA> (L p) empty {}.), [{AStop}], {}., \<abinit>))})" (is "finite ?S")
+proof (rule finite_subset[OF _finite_arg_space])
+  have [simp]:"p \<in> lambdas p" by (cases p, simp)
+  show "?S \<subseteq> arg_poss p"
+  by  (rule UN_iterate_less[OF _ arg_space_complete_ps])
+      (auto simp add:arg_poss_def fstate_poss_def proc_poss_def call_list_lengths_def NList_def nList_def
+         intro!: imageI)
+qed
 
 lemma Un_commute_helper:"(a \<union> b) \<union> (c \<union> d) = (a \<union> c) \<union> (b \<union> d)"
 by auto
