CFGraph/CPSUtils.thy
@@ -12,6 +12,7 @@ where "lambdas  (Lambda l vs c) = ({Lambda l vs c} \<union> lambdasC c)"
     | "lambdasV (L l) = lambdas l"
     | "lambdasV _     = {}"
 
+
 fun calls :: "lambda \<Rightarrow> call set"
 and callsC :: "call \<Rightarrow> call set"
 and callsV :: "val \<Rightarrow> call set"
@@ -22,6 +23,34 @@ where "calls  (Lambda l vs c) = callsC c"
                                     \<union> callsC c')"
     | "callsV (L l) = calls l"
     | "callsV _     = {}"
+
+
+inductive_set lambdas' and calls' and values'
+  for p
+  where "p \<in> lambdas' p"
+      | "Lambda l vs c \<in> lambdas' p \<Longrightarrow> c \<in> calls' p"
+      | "App l d ds \<in> calls' p \<Longrightarrow> d \<in> values' p"
+      | "\<lbrakk> App l d ds \<in> calls' p ; d' \<in> set ds \<rbrakk> \<Longrightarrow> d' \<in> values' p"
+      | "Let l binds c' \<in> calls' p \<Longrightarrow> c' \<in> calls' p"
+      | "\<lbrakk> Let l binds c' \<in> calls' p ; l' \<in> snd ` set binds \<rbrakk> \<Longrightarrow> l' \<in> lambdas' p"
+      | "L l \<in> values' p \<Longrightarrow> l \<in> lambdas' p"
+
+(* thm  lambdas'p_calls'p_values'p_def *)
+
+
+(*
+lemma "l \<in> lambdas' p \<Longrightarrow> l \<in> lambdas p" and "c \<in> calls' p \<Longrightarrow> c \<in> calls p" and "v \<in> values' p \<Longrightarrow> True"
+(* apply (rule lambdas_lambdasC_lambdasV.induct) *)
+(* apply (auto intro: lambdas'_calls'_values'.intros) *)
+thm lambdas'_calls'_values'.inducts
+apply (induct rule: lambdas'_calls'_values'.inducts)
+
+lemma "l \<in> lambdas p \<Longrightarrow> l \<in> lambdas' p" and "l \<in> lambdas p \<Longrightarrow> l \<in> lambdas' p"
+thm lambdas_lambdasC_lambdasV.induct
+apply (induct rule: lambdas_lambdasC_lambdasV.induct)
+apply auto
+*)
+
 
 lemma finite_lambdas[simp]: "finite (lambdas l)" and "finite (lambdasC c)" "finite (lambdasV v)"
 by (induct rule: lambdas_lambdasC_lambdasV.induct, auto, blast)
@@ -51,14 +80,203 @@ fun labels :: "lambda \<Rightarrow> label set"
 and labelsC :: "call \<Rightarrow> label set"
 and labelsV :: "val \<Rightarrow> label set"
 where "labels (Lambda l vs c) = {l} \<union> labelsC c"
-    | "labelsC (App l a as) = {l} \<union> UNION (set as) labelsV"
-    | "labelsC (Let _ binds c') = UNION (set binds) (\<lambda>(v,l). labels l) \<union> labelsC c'"
+    | "labelsC (App l a as) = {l} \<union> labelsV a \<union> UNION (set as) labelsV"
+    | "labelsC (Let l binds c') = {l} \<union> UNION (set binds) (\<lambda>(v,l). labels l) \<union> labelsC c'"
     | "labelsV (L l) = labels l"
     | "labelsV (R l _) = {l}"
     | "labelsV _  = {}"
 
 lemma finite_labels[simp]: "finite (labels l)" and "finite (labelsC c)" "finite (labelsV v)"
 by (induct rule: labels_labelsC_labelsV.induct, auto, blast)
+
+fun prims :: "lambda \<Rightarrow> prim set"
+and primsC :: "call \<Rightarrow> prim set"
+and primsV :: "val \<Rightarrow> prim set"
+where "prims (Lambda _ vs c) = primsC c"
+    | "primsC (App _ a as) = primsV a \<union> UNION (set as) primsV"
+    | "primsC (Let _ binds c') = UNION (set binds) (\<lambda>(_,l). prims l) \<union> primsC c'"
+    | "primsV (L l) = prims l"
+    | "primsV (R l v) = {}"
+    | "primsV (P prim) = {prim}"
+    | "primsV (C l v) = {}"
+
+lemma finite_prims[simp]: "finite (prims l)" and "finite (primsC c)" "finite (primsV v)"
+by (induct rule: labels_labelsC_labelsV.induct, auto, blast)
+
+fun vals :: "lambda \<Rightarrow> val set"
+and valsC :: "call \<Rightarrow> val set"
+and valsV :: "val \<Rightarrow> val set"
+where "vals (Lambda _ vs c) = valsC c"
+    | "valsC (App _ a as) = valsV a \<union> UNION (set as) valsV"
+    | "valsC (Let _ binds c') = UNION (set binds) (\<lambda>(_,l). vals l) \<union> valsC c'"
+    | "valsV (L l) = {L l} \<union> vals l"
+    | "valsV (R l v) = {R l v}"
+    | "valsV (P prim) = {P prim}"
+    | "valsV (C l v) = {C l v}"
+
+
+thm lambda_call_val.inducts
+
+lemma 
+  shows lambdas1: "Lambda l vs c \<in> lambdas x \<Longrightarrow> c \<in> calls x"
+  and "Lambda l vs c \<in> lambdasC y \<Longrightarrow> c \<in> callsC y"
+  and "Lambda l vs c \<in> lambdasV z \<Longrightarrow> c \<in> callsV z"
+  and "\<forall>z\<in> set list. Lambda l vs c \<in> lambdasV z \<longrightarrow> c \<in> callsV z"
+  and "\<forall>x\<in> set (list2 :: (var \<times> lambda) list) . Lambda l vs c \<in> lambdas (snd x) \<longrightarrow> c \<in> calls (snd x)"
+  and "Lambda l vs c \<in> lambdas (snd (t:: var\<times>lambda)) \<Longrightarrow> c \<in> calls (snd t)"
+apply (induct rule:lambda_call_val.inducts)
+apply auto
+apply (case_tac c, auto)[1]
+apply (rule_tac x="((a, b), ba)" in bexI, auto)
+done
+
+lemma 
+  shows lambdas2: "Lambda l vs c \<in> lambdas x \<Longrightarrow> l \<in> labels x"
+  and "Lambda l vs c \<in> lambdasC y \<Longrightarrow> l \<in> labelsC y"
+  and "Lambda l vs c \<in> lambdasV z \<Longrightarrow> l \<in> labelsV z"
+  and "\<forall>z\<in> set list. Lambda l vs c \<in> lambdasV z \<longrightarrow> l \<in> labelsV z"
+  and "\<forall>x\<in> set (list2 :: (var \<times> lambda) list) . Lambda l vs c \<in> lambdas (snd x) \<longrightarrow> l \<in> labels (snd x)"
+  and "Lambda l vs c \<in> lambdas (snd (t:: var\<times>lambda)) \<Longrightarrow> l \<in> labels (snd t)"
+apply (induct rule:lambda_call_val.inducts)
+apply auto
+apply (rule_tac x="((a, b), ba)" in bexI, auto)
+done
+
+lemma 
+  shows lambdas3: "Lambda l vs c \<in> lambdas x \<Longrightarrow> set vs \<subseteq> vars x"
+  and "Lambda l vs c \<in> lambdasC y \<Longrightarrow> set vs \<subseteq> varsC y"
+  and "Lambda l vs c \<in> lambdasV z \<Longrightarrow> set vs \<subseteq> varsV z"
+  and "\<forall>z\<in> set list. Lambda l vs c \<in> lambdasV z \<longrightarrow> set vs \<subseteq> varsV z"
+  and "\<forall>x\<in> set (list2 :: (var \<times> lambda) list) . Lambda l vs c \<in> lambdas (snd x) \<longrightarrow> set vs \<subseteq> vars (snd x)"
+  and "Lambda l vs c \<in> lambdas (snd (t:: var\<times>lambda)) \<Longrightarrow> set vs \<subseteq> vars (snd t)"
+apply (induct x and y and z and list and list2 and t rule:lambda_call_val.inducts)
+apply auto
+apply (erule_tac x="((aa, ba), bb)" in ballE)
+apply (rule_tac x="((aa, ba), bb)" in bexI, auto)
+done
+
+lemma 
+  shows app1: "App l d ds \<in> calls x \<Longrightarrow> d \<in> vals x"
+  and "App l d ds \<in> callsC y \<Longrightarrow> d \<in> valsC y"
+  and "App l d ds \<in> callsV z \<Longrightarrow> d \<in> valsV z"
+  and "\<forall>z\<in> set list. App l d ds \<in> callsV z \<longrightarrow> d \<in> valsV z"
+  and "\<forall>x\<in> set (list2 :: (var \<times> lambda) list) . App l d ds \<in> calls (snd x) \<longrightarrow> d \<in> vals (snd x)"
+  and "App l d ds \<in> calls (snd (t:: var\<times>lambda)) \<Longrightarrow> d \<in> vals (snd t)"
+apply (induct  x and y and z and list and list2 and t rule:lambda_call_val.inducts)
+apply auto
+apply (case_tac d, auto)
+apply (erule_tac x="((a, b), ba)" in ballE)
+apply (rule_tac x="((a, b), ba)" in bexI, auto)
+done
+
+lemma 
+  shows app2: "App l d ds \<in> calls x \<Longrightarrow> set ds \<subseteq> vals x"
+  and "App l d ds \<in> callsC y \<Longrightarrow> set ds \<subseteq> valsC y"
+  and "App l d ds \<in> callsV z \<Longrightarrow> set ds \<subseteq> valsV z"
+  and "\<forall>z\<in> set list. App l d ds \<in> callsV z \<longrightarrow> set ds \<subseteq> valsV z"
+  and "\<forall>x\<in> set (list2 :: (var \<times> lambda) list) . App l d ds \<in> calls (snd x) \<longrightarrow> set ds \<subseteq> vals (snd x)"
+  and "App l d ds \<in> calls (snd (t:: var\<times>lambda)) \<Longrightarrow> set ds \<subseteq> vals (snd t)"
+apply (induct  x and y and z and list and list2 and t rule:lambda_call_val.inducts)
+apply auto
+apply (case_tac x, auto)
+apply (erule_tac x="((a, b), ba)" in ballE)
+apply (rule_tac x="((a, b), ba)" in bexI, auto)
+done
+
+lemma 
+  shows let1: "Let l binds c' \<in> calls x \<Longrightarrow> l \<in> labels x"
+  and "Let l binds c' \<in> callsC y \<Longrightarrow> l \<in> labelsC y"
+  and "Let l binds c' \<in> callsV z \<Longrightarrow> l \<in> labelsV z"
+  and "\<forall>z\<in> set list. Let l binds c' \<in> callsV z \<longrightarrow> l \<in> labelsV z"
+  and "\<forall>x\<in> set (list2 :: (var \<times> lambda) list) . Let l binds c' \<in> calls (snd x) \<longrightarrow> l \<in> labels (snd x)"
+  and "Let l binds c' \<in> calls (snd (t:: var\<times>lambda)) \<Longrightarrow> l \<in> labels (snd t)"
+apply (induct x and y and z and list and list2 and t rule:lambda_call_val.inducts)
+apply auto
+apply (erule_tac x="((a, b), ba)" in ballE)
+apply (rule_tac x="((a, b), ba)" in bexI, auto)
+done
+
+lemma 
+  shows let2: "Let l binds c' \<in> calls x \<Longrightarrow> c' \<in> calls x"
+  and "Let l binds c' \<in> callsC y \<Longrightarrow> c' \<in> callsC y"
+  and "Let l binds c' \<in> callsV z \<Longrightarrow> c' \<in> callsV z"
+  and "\<forall>z\<in> set list. Let l binds c' \<in> callsV z \<longrightarrow> c' \<in> callsV z"
+  and "\<forall>x\<in> set (list2 :: (var \<times> lambda) list) . Let l binds c' \<in> calls (snd x) \<longrightarrow> c' \<in> calls (snd x)"
+  and "Let l binds c' \<in> calls (snd (t:: var\<times>lambda)) \<Longrightarrow> c' \<in> calls (snd t)"
+apply (induct x and y and z and list and list2 and t rule:lambda_call_val.inducts)
+apply auto
+apply (case_tac c', auto)
+apply (erule_tac x="((a, b), ba)" in ballE)
+apply (rule_tac x="((a, b), ba)" in bexI, auto)
+done
+
+lemma 
+  shows let3: "Let l binds c' \<in> calls x \<Longrightarrow> fst ` set binds \<subseteq> vars x"
+  and "Let l binds c' \<in> callsC y \<Longrightarrow> fst ` set binds \<subseteq> varsC y"
+  and "Let l binds c' \<in> callsV z \<Longrightarrow> fst ` set binds \<subseteq> varsV z"
+  and "\<forall>z\<in> set list. Let l binds c' \<in> callsV z \<longrightarrow> fst ` set binds \<subseteq> varsV z"
+  and "\<forall>x\<in> set (list2 :: (var \<times> lambda) list) . Let l binds c' \<in> calls (snd x) \<longrightarrow> fst ` set binds \<subseteq> vars (snd x)"
+  and "Let l binds c' \<in> calls (snd (t:: var\<times>lambda)) \<Longrightarrow> fst ` set binds \<subseteq> vars (snd t)"
+apply (induct x and y and z and list and list2 and t rule:lambda_call_val.inducts)
+apply auto
+apply (erule_tac x="((ab, bc), bd)" in ballE)
+apply (rule_tac x="((ab, bc), bd)" in bexI, auto)
+done
+
+lemma
+  shows let4: "Let l binds c' \<in> calls x \<Longrightarrow> snd ` set binds \<subseteq> lambdas x"
+  and "Let l binds c' \<in> callsC y \<Longrightarrow> snd ` set binds \<subseteq> lambdasC y"
+  and "Let l binds c' \<in> callsV z \<Longrightarrow> snd ` set binds \<subseteq> lambdasV z"
+  and "\<forall>z\<in> set list. Let l binds c' \<in> callsV z \<longrightarrow> snd ` set binds \<subseteq> lambdasV z"
+  and "\<forall>x\<in> set (list2 :: (var \<times> lambda) list) . Let l binds c' \<in> calls (snd x) \<longrightarrow> snd ` set binds \<subseteq> lambdas (snd x)"
+  and "Let l binds c' \<in> calls (snd (t:: var\<times>lambda)) \<Longrightarrow> snd ` set binds \<subseteq> lambdas (snd t)"
+apply (induct x and y and z and list and list2 and t rule:lambda_call_val.inducts)
+apply auto
+apply (rule_tac x="((a, b), ba)" in bexI, auto)
+apply (case_tac ba, auto)
+apply (erule_tac x="((aa, bb), bc)" in ballE)
+apply (rule_tac x="((aa, bb), bc)" in bexI, auto)
+done
+
+lemma
+shows vals1: "P prim \<in> vals p \<Longrightarrow> prim \<in> prims p"
+  and "P prim \<in> valsC y \<Longrightarrow> prim \<in> primsC y"
+  and "P prim \<in> valsV z \<Longrightarrow> prim \<in> primsV z"
+  and "\<forall>z\<in> set list. P prim \<in> valsV z \<longrightarrow> prim \<in> primsV z"
+  and "\<forall>x\<in> set (list2 :: (var \<times> lambda) list) . P prim \<in> vals (snd x) \<longrightarrow> prim \<in> prims (snd x)"
+  and "P prim \<in> vals (snd (t:: var\<times>lambda)) \<Longrightarrow> prim \<in> prims (snd t)"
+apply (induct rule:lambda_call_val.inducts)
+apply auto
+apply (erule_tac x="((a, b), ba)" in ballE)
+apply (rule_tac x="((a, b), ba)" in bexI, auto)
+done
+
+lemma
+shows vals2: "R l var \<in> vals p \<Longrightarrow> var \<in> vars p"
+  and "R l var \<in> valsC y \<Longrightarrow> var \<in> varsC y"
+  and "R l var \<in> valsV z \<Longrightarrow> var \<in> varsV z"
+  and "\<forall>z\<in> set list. R l var \<in> valsV z \<longrightarrow> var \<in> varsV z"
+  and "\<forall>x\<in> set (list2 :: (var \<times> lambda) list) . R l var \<in> vals (snd x) \<longrightarrow> var \<in> vars (snd x)"
+  and "R l var \<in> vals (snd (t:: var\<times>lambda)) \<Longrightarrow> var \<in> vars (snd t)"
+apply (induct rule:lambda_call_val.inducts)
+apply auto
+apply (erule_tac x="((a, b), ba)" in ballE)
+apply (rule_tac x="((a, b), ba)" in bexI, auto)
+done
+
+lemma
+shows vals3: "L l \<in> vals p \<Longrightarrow> l \<in> lambdas p"
+  and "L l \<in> valsC y \<Longrightarrow> l \<in> lambdasC y"
+  and "L l \<in> valsV z \<Longrightarrow> l \<in> lambdasV z"
+  and "\<forall>z\<in> set list. L l \<in> valsV z \<longrightarrow> l \<in> lambdasV z"
+  and "\<forall>x\<in> set (list2 :: (var \<times> lambda) list) . L l \<in> vals (snd x) \<longrightarrow> l \<in> lambdas (snd x)"
+  and "L l \<in> vals (snd (t:: var\<times>lambda)) \<Longrightarrow> l \<in> lambdas (snd t)"
+apply (induct rule:lambda_call_val.inducts)
+apply auto
+apply (erule_tac x="((a, b), ba)" in ballE)
+apply (rule_tac x="((a, b), ba)" in bexI, auto)
+apply (case_tac l, auto)
+done
 
 
 definition nList :: "'a set => nat => 'a list set"
@@ -90,7 +308,7 @@ lemma finite_Nlist[intro]:
 unfolding NList_def using assms by auto
 
 definition call_list_lengths
-  where "call_list_lengths p = (\<lambda>c. case c of (App _ _ ds) \<Rightarrow> length ds | _ \<Rightarrow> 0) ` calls p"
+  where "call_list_lengths p = {0,1,2,3} \<union> (\<lambda>c. case c of (App _ _ ds) \<Rightarrow> length ds | _ \<Rightarrow> 0) ` calls p"
 
 lemma finite_call_list_lengths[simp]: "finite (call_list_lengths p)"
   unfolding call_list_lengths_def by auto
